<?xml version="1.0"?>
<rdf:RDF xmlns="http://www.w3.org/ns/sosa/"
     xml:base="http://www.w3.org/ns/sosa/"
     xmlns:schema="http://schema.org/"
     xmlns:dct="http://purl.org/dc/terms/"
     xmlns:rdf="http://www.w3.org/1999/02/22-rdf-syntax-ns#"
     xmlns:owl="http://www.w3.org/2002/07/owl#"
     xmlns:xml="http://www.w3.org/XML/1998/namespace"
     xmlns:xsd="http://www.w3.org/2001/XMLSchema#"
     xmlns:skos="http://www.w3.org/2004/02/skos/core#"
     xmlns:rdfs="http://www.w3.org/2000/01/rdf-schema#"
     xmlns:vann="http://purl.org/vocab/vann/"
     xmlns:foaf="http://xmlns.com/foaf/0.1/"
     xmlns:dc="http://purl.org/dc/elements/1.1/">
    <owl:Ontology rdf:about="http://www.w3.org/ns/sosa/">
        <owl:versionIRI rdf:resource="http://vocab.ciudadesabiertas.es/def/medio-ambiente/contaminacion-acustica"/>
        <owl:imports rdf:resource="http://www.w3.org/ns/sosa/"/>
        <vann:preferredNamespaceUri rdf:resource="http://vocab.ciudadesabiertas.es/def/medio-ambiente/contaminacion-acustica#"/>
        <dc:contributor xml:lang="es">Red.es</dc:contributor>
        <dc:creator>Paola Espinoza Arias (Ontology Engineering Group - Universidad Politécnica de Madrid)</dc:creator>
        <dc:contributor xml:lang="es">María Jesús Gallego San Miguel - Ayuntamiento de Madrid</dc:contributor>
        <dct:license rdf:resource="https://creativecommons.org/licenses/by/4.0"/>
        <dc:contributor xml:lang="es">Servicio de Informática - Ayuntamiento de Santiago de Compostela</dc:contributor>
        <vann:preferredNamespacePrefix>noise</vann:preferredNamespacePrefix>
        <dc:identifier rdf:resource="http://vocab.ciudadesabiertas.es/def/medio-ambiente/contaminacion-acustica"/>
        <owl:priorVersion rdf:resource="http://vocab.linkeddata.es/datosabiertos/def/medio-ambiente/contaminacion-acustica"/>
        <dc:contributor xml:lang="es">María Carmen Ruiz Moreno - Ayuntamiento de Madrid</dc:contributor>
        <dc:contributor xml:lang="es">María Jesús Fernández Ruiz - Ayuntamiento de Zaragoza</dc:contributor>
        <owl:versionInfo>Esta es la versión inicial de la ontología de Contaminación Acústica que ha sido implementada en el contexto del proyecto &quot;Plataforma de gobierno abierto, colaborativa e interoperable&quot; en la que participan los ayuntamientos de Madrid, Zaragoza, Santiago de Compostela y La Coruña.</owl:versionInfo>
        <dc:creator>Francisco Yedro (Ontology Engineering Group - Universidad Politécnica de Madrid)</dc:creator>
        <dc:title xml:lang="en">Vocabulary for the representation of data about noise pollution</dc:title>
        <dc:contributor xml:lang="es">María del Mar Arribas de Andrés - Ayuntamiento de Madrid</dc:contributor>
        <rdfs:comment xml:lang="es">Esta versión ha sido generada dentro del contexto del proyecto &quot;Plataforma de gobierno abierto, colaborativa e interoperable&quot; en el que participan los ayuntamientos de Madrid, Zaragoza, Santiago de Compostela y A Coruña.
En esta versión se han incluido clases y propiedades de acuerdo a los requisitos y glosario de conceptos propuestos en la reunión del 07/11/2019</rdfs:comment>
        <dct:issued xml:lang="es">2019-11-07</dct:issued>
        <dc:title xml:lang="es">Vocabulario para la representación de datos sobre el sistema de contaminación acústica</dc:title>
        <dc:contributor xml:lang="es">Servicio de Innovación y Desarrollo Tecnológico - Ayuntamiento de A Coruña</dc:contributor>
        <dc:creator>Edna Ruckhaus (Ontology Engineering Group - Universidad Politécnica de Madrid)</dc:creator>
        <dc:creator>Oscar Corcho (Ontology Engineering Group - Universidad Politécnica de Madrid, Localidata)</dc:creator>
        <dc:contributor xml:lang="es">Honorio Enrique Crespo Díaz-Alejo - Ayuntamiento de Madrid</dc:contributor>
        <dc:contributor xml:lang="es">Víctor Morlán Plo - Ayuntamiento de Zaragoza</dc:contributor>
    </owl:Ontology>
    


    <!-- 
    ///////////////////////////////////////////////////////////////////////////////////////
    //
    // Annotation properties
    //
    ///////////////////////////////////////////////////////////////////////////////////////
     -->

    


    <!-- http://purl.org/dc/elements/1.1/contributor -->

    <owl:AnnotationProperty rdf:about="http://purl.org/dc/elements/1.1/contributor"/>
    


    <!-- http://purl.org/dc/elements/1.1/creator -->

    <owl:AnnotationProperty rdf:about="http://purl.org/dc/elements/1.1/creator"/>
    


    <!-- http://purl.org/dc/elements/1.1/date -->

    <owl:AnnotationProperty rdf:about="http://purl.org/dc/elements/1.1/date"/>
    


    <!-- http://purl.org/dc/elements/1.1/identifier -->

    <owl:AnnotationProperty rdf:about="http://purl.org/dc/elements/1.1/identifier"/>
    


    <!-- http://purl.org/dc/elements/1.1/title -->

    <owl:AnnotationProperty rdf:about="http://purl.org/dc/elements/1.1/title"/>
    


    <!-- http://purl.org/dc/terms/hasVersion -->

    <owl:AnnotationProperty rdf:about="http://purl.org/dc/terms/hasVersion"/>
    


    <!-- http://purl.org/dc/terms/issued -->

    <owl:AnnotationProperty rdf:about="http://purl.org/dc/terms/issued">
        <dct:hasVersion rdf:resource="http://dublincore.org/usage/terms/history/#issued-003"/>
        <rdfs:comment xml:lang="en">Date of formal issuance (e.g., publication) of the resource.</rdfs:comment>
        <rdfs:isDefinedBy xml:lang="en">http://purl.org/dc/terms/</rdfs:isDefinedBy>
        <rdfs:label xml:lang="en">Date Issued</rdfs:label>
        <rdfs:subPropertyOf rdf:resource="http://purl.org/dc/elements/1.1/date"/>
    </owl:AnnotationProperty>
    


    <!-- http://purl.org/dc/terms/license -->

    <owl:AnnotationProperty rdf:about="http://purl.org/dc/terms/license"/>
    


    <!-- http://schema.org/domainIncludes -->

    <owl:AnnotationProperty rdf:about="http://schema.org/domainIncludes"/>
    


    <!-- http://www.w3.org/2004/02/skos/core#definition -->

    <owl:AnnotationProperty rdf:about="http://www.w3.org/2004/02/skos/core#definition"/>
    


    <!-- http://www.w3.org/2004/02/skos/core#example -->

    <owl:AnnotationProperty rdf:about="http://www.w3.org/2004/02/skos/core#example"/>
    


    <!-- http://www.w3.org/ns/sosa/hasSimpleResult -->

    <owl:AnnotationProperty rdf:about="http://www.w3.org/ns/sosa/hasSimpleResult">
        <rdfs:range rdf:resource="http://www.w3.org/2000/01/rdf-schema#Literal"/>
        <rdfs:domain rdf:resource="http://vocab.ciudadesabiertas.es/def/medio-ambiente/contaminacion-acustica#Observacion"/>
        <rdfs:domain rdf:resource="http://www.w3.org/ns/sosa/Observation"/>
    </owl:AnnotationProperty>
    


    <!-- http://www.w3.org/ns/sosa/resultTime -->

    <owl:AnnotationProperty rdf:about="http://www.w3.org/ns/sosa/resultTime">
        <rdfs:range rdf:resource="http://www.w3.org/2001/XMLSchema#dateTime"/>
        <rdfs:domain rdf:resource="http://vocab.ciudadesabiertas.es/def/medio-ambiente/contaminacion-acustica#Observacion"/>
        <rdfs:domain rdf:resource="http://www.w3.org/ns/sosa/Observation"/>
    </owl:AnnotationProperty>
    


    <!-- 
    ///////////////////////////////////////////////////////////////////////////////////////
    //
    // Datatypes
    //
    ///////////////////////////////////////////////////////////////////////////////////////
     -->

    


    <!-- http://www.w3.org/2001/XMLSchema#date -->

    <rdfs:Datatype rdf:about="http://www.w3.org/2001/XMLSchema#date"/>
    


    <!-- 
    ///////////////////////////////////////////////////////////////////////////////////////
    //
    // Object Properties
    //
    ///////////////////////////////////////////////////////////////////////////////////////
     -->

    


    <!-- http://schema.org/address -->

    <owl:ObjectProperty rdf:about="http://schema.org/address">
        <rdfs:domain rdf:resource="http://vocab.ciudadesabiertas.es/def/medio-ambiente/contaminacion-acustica#EstacionMedida"/>
        <rdfs:range rdf:resource="http://schema.org/PostalAddress"/>
        <rdfs:isDefinedBy rdf:resource="http://schema.org/"/>
        <rdfs:label xml:lang="en">address</rdfs:label>
        <rdfs:label xml:lang="es">dirección</rdfs:label>
    </owl:ObjectProperty>
    


    <!-- http://vocab.ciudadesabiertas.es/def/medio-ambiente/contaminacion-acustica#tipoEmisorPredominante -->

    <owl:ObjectProperty rdf:about="http://vocab.ciudadesabiertas.es/def/medio-ambiente/contaminacion-acustica#tipoEmisorPredominante">
        <rdfs:domain rdf:resource="http://vocab.ciudadesabiertas.es/def/medio-ambiente/contaminacion-acustica#Observacion"/>
        <rdfs:range>
            <owl:Class>
                <owl:intersectionOf rdf:parseType="Collection">
                    <rdf:Description rdf:about="http://www.w3.org/2004/02/skos/core#Concept"/>
                    <owl:Restriction>
                        <owl:onProperty rdf:resource="http://www.w3.org/2004/02/skos/core#inScheme"/>
                        <owl:hasValue rdf:resource="http://vocab.linkeddata.es/datosabiertos/kos/medio-ambiente/contaminacion-acustica/tipo-emisor-predominante"/>
                    </owl:Restriction>
                </owl:intersectionOf>
            </owl:Class>
        </rdfs:range>
        <rdfs:comment xml:lang="es">El tipo de emisor está basado en en el listado obtenido en el artículo 12.2 de la Ley 37/2003, de 17 de noviembre, del Ruido.
a) Vehículos automóviles.
b) Ferrocarriles.
c) Aeronaves.
d) Infraestructuras viarias.
e) Infraestructuras ferroviarias.
f) Infraestructuras aeroportuarias.
g) Maquinaria y equipos.
h) Obras de construcción de edificios y de ingeniería civil.
i) Actividades industriales.
j) Actividades comerciales.
k) Actividades deportivo-recreativas y de ocio.
l) Infraestructuras portuarias.</rdfs:comment>
        <rdfs:comment xml:lang="en">The type of emitter is based on the list obtained in article 12.2 of Law 37/2003, of November 17, on Noise.
a) Motor vehicles.
b) Railways.
c) Aircraft.
d) Road infrastructure.
e) Railway infrastructure.
f) Airport infrastructure.
g) Machinery and equipment.
h) Building construction and civil engineering works.
i) Industrial activities.
j) Commercial activities.
k) Sports-recreational and leisure activities.
l) Port infrastructure.</rdfs:comment>
        <rdfs:isDefinedBy rdf:resource="http://vocab.ciudadesabiertas.es/def/medio-ambiente/contaminacion-acustica"/>
        <rdfs:label xml:lang="en">predominant type of emitter</rdfs:label>
        <rdfs:label xml:lang="es">tipo de emisor predominante</rdfs:label>
    </owl:ObjectProperty>
    


    <!-- http://vocab.ciudadesabiertas.es/def/medio-ambiente/contaminacion-acustica#tipoIntervaloReferencia -->

    <owl:ObjectProperty rdf:about="http://vocab.ciudadesabiertas.es/def/medio-ambiente/contaminacion-acustica#tipoIntervaloReferencia">
        <rdfs:domain rdf:resource="http://vocab.ciudadesabiertas.es/def/medio-ambiente/contaminacion-acustica#Observacion"/>
        <rdfs:range>
            <owl:Class>
                <owl:intersectionOf rdf:parseType="Collection">
                    <rdf:Description rdf:about="http://www.w3.org/2004/02/skos/core#Concept"/>
                    <owl:Restriction>
                        <owl:onProperty rdf:resource="http://www.w3.org/2004/02/skos/core#inScheme"/>
                        <owl:hasValue rdf:resource="http://vocab.linkeddata.es/datosabiertos/kos/medio-ambiente/contaminacion-acustica/tipo-intervalo-referencia"/>
                    </owl:Restriction>
                </owl:intersectionOf>
            </owl:Class>
        </rdfs:range>
        <rdfs:comment xml:lang="es">Basado en cuatro tipos:
(T, total, D diurno, E tarde, N noche)
Lden - Indicador del nivel de ruido global durante el día, la tarde y la noche, utilizado para determinar la molestia vinculada a la exposición al ruido.
Ld - Nivel sonoro medio a largo plazo ponderado A, determinado a lo largo de todos los períodos día (de 7 a 19 horas) del mes.
Le - Nivel sonoro medio a largo plazo ponderado A, determinado a lo largo de todos los períodos tarde (de 19 a 23 horas) del mes.
Ln - Nivel sonoro medio a largo plazo ponderado A, definido determinado a lo largo de todos los períodos noche (de 23 a 7 horas) del mes.</rdfs:comment>
        <rdfs:comment xml:lang="en">Based on four types:
(T, total, D daytime, E afternoon, N night)
Lden - Indicator of overall noise level during the day, afternoon, and night, used to determine nuisance related to noise exposure.
Ld - A-weighted long-term average sound level, determined throughout all day periods (from 7 to 19 hours) of the month.
Le - A-weighted long-term average sound level, determined throughout all the late periods (from 19 to 23 hours) of the month.
Ln - A-weighted long-term average sound level, defined determined throughout all night periods (23 to 7 hours) of the month.</rdfs:comment>
        <rdfs:isDefinedBy rdf:resource="http://vocab.ciudadesabiertas.es/def/medio-ambiente/contaminacion-acustica"/>
        <rdfs:label xml:lang="en">reference interval type</rdfs:label>
        <rdfs:label xml:lang="es">tipo de intervalo de referencia</rdfs:label>
    </owl:ObjectProperty>
    


    <!-- http://vocab.ciudadesabiertas.es/def/medio-ambiente/contaminacion-acustica#tipoMedida -->

    <owl:ObjectProperty rdf:about="http://vocab.ciudadesabiertas.es/def/medio-ambiente/contaminacion-acustica#tipoMedida">
        <rdfs:domain rdf:resource="http://vocab.ciudadesabiertas.es/def/medio-ambiente/contaminacion-acustica#Observacion"/>
        <rdfs:range>
            <owl:Class>
                <owl:intersectionOf rdf:parseType="Collection">
                    <rdf:Description rdf:about="http://www.w3.org/2004/02/skos/core#Concept"/>
                    <owl:Restriction>
                        <owl:onProperty rdf:resource="http://www.w3.org/2004/02/skos/core#inScheme"/>
                        <owl:hasValue rdf:resource="http://vocab.linkeddata.es/datosabiertos/kos/medio-ambiente/contaminacion-acustica/tipo-medicion"/>
                    </owl:Restriction>
                </owl:intersectionOf>
            </owl:Class>
        </rdfs:range>
        <rdfs:comment xml:lang="es">Cada medición puede tener los siguientes tipos LAeq, LAs01, LAs10, LAs50, LAs90, LAs99. Numérico, 5 dígitos. También puede ser LAw para medir posibles vibraciones.</rdfs:comment>
        <rdfs:comment xml:lang="en">Each measurement can have the following types LAeq, LAs01, LAs10, LAs50, LAs90, LAs99. Numeric, 5 digits. It can also be LAw to measure possible vibrations.</rdfs:comment>
        <rdfs:isDefinedBy rdf:resource="http://vocab.ciudadesabiertas.es/def/medio-ambiente/contaminacion-acustica"/>
        <rdfs:label xml:lang="en">measurement type</rdfs:label>
        <rdfs:label xml:lang="es">tipo de medición</rdfs:label>
    </owl:ObjectProperty>
    


    <!-- http://vocab.linkeddata.es/datosabiertos/def/urbanismo-infraestructuras/equipamiento-municipal#tipoEquipamiento -->

    <owl:ObjectProperty rdf:about="http://vocab.linkeddata.es/datosabiertos/def/urbanismo-infraestructuras/equipamiento-municipal#tipoEquipamiento">
        <rdfs:domain rdf:resource="http://vocab.linkeddata.es/datosabiertos/def/urbanismo-infraestructuras/equipamiento-municipal#Equipamiento"/>
    </owl:ObjectProperty>
    


    <!-- http://www.w3.org/2004/02/skos/core#inScheme -->

    <owl:ObjectProperty rdf:about="http://www.w3.org/2004/02/skos/core#inScheme">
        <rdfs:range rdf:resource="http://www.w3.org/2004/02/skos/core#ConceptScheme"/>
        <rdfs:isDefinedBy rdf:resource="http://www.w3.org/2004/02/skos/core"/>
        <rdfs:label xml:lang="en">is in scheme</rdfs:label>
        <skos:definition xml:lang="en">Relates a resource (for example a concept) to a concept scheme in which it is included.</skos:definition>
    </owl:ObjectProperty>
    


    <!-- http://www.w3.org/ns/sosa/madeBySensor -->

    <owl:ObjectProperty rdf:about="http://www.w3.org/ns/sosa/madeBySensor"/>
    


    <!-- http://www.w3.org/ns/sosa/observedProperty -->

    <owl:ObjectProperty rdf:about="http://www.w3.org/ns/sosa/observedProperty"/>
    


    <!-- http://www.w3.org/ns/sosa/observes -->

    <owl:ObjectProperty rdf:about="http://www.w3.org/ns/sosa/observes"/>
    


    <!-- 
    ///////////////////////////////////////////////////////////////////////////////////////
    //
    // Data properties
    //
    ///////////////////////////////////////////////////////////////////////////////////////
     -->

    


    <!-- http://purl.org/dc/terms/identifier -->

    <owl:DatatypeProperty rdf:about="http://purl.org/dc/terms/identifier">
        <rdfs:domain rdf:resource="http://vocab.linkeddata.es/datosabiertos/def/urbanismo-infraestructuras/equipamiento-municipal#Equipamiento"/>
        <rdfs:range rdf:resource="http://www.w3.org/2001/XMLSchema#string"/>
        <rdfs:comment xml:lang="en">An unambiguous reference to the resource within a given context.</rdfs:comment>
        <rdfs:comment xml:lang="es">Referencia inequívoca al recurso dentro de un contexto dado.</rdfs:comment>
        <rdfs:isDefinedBy rdf:resource="http://purl.org/dc/terms/"/>
        <rdfs:label xml:lang="es">Identificador</rdfs:label>
        <rdfs:label xml:lang="en">Identifier</rdfs:label>
    </owl:DatatypeProperty>
    


    <!-- http://schema.org/addressCountry -->

    <owl:DatatypeProperty rdf:about="http://schema.org/addressCountry">
        <rdfs:domain rdf:resource="http://schema.org/PostalAddress"/>
    </owl:DatatypeProperty>
    


    <!-- http://schema.org/addressLocality -->

    <owl:DatatypeProperty rdf:about="http://schema.org/addressLocality">
        <rdfs:domain rdf:resource="http://schema.org/PostalAddress"/>
        <rdfs:range rdf:resource="http://www.w3.org/2001/XMLSchema#string"/>
        <rdfs:comment xml:lang="es">La localidad. Por ejemplo, Zaragoza</rdfs:comment>
        <rdfs:isDefinedBy rdf:resource="http://schema.org/"/>
        <rdfs:label xml:lang="es">localidad</rdfs:label>
    </owl:DatatypeProperty>
    


    <!-- http://schema.org/addressRegion -->

    <owl:DatatypeProperty rdf:about="http://schema.org/addressRegion">
        <rdfs:domain rdf:resource="http://schema.org/PostalAddress"/>
        <rdfs:range rdf:resource="http://www.w3.org/2001/XMLSchema#string"/>
        <rdfs:comment xml:lang="es">La región. Por ejemplo, Provincia de Zaragoza o Comunidad Autónoma de Aragón</rdfs:comment>
        <rdfs:isDefinedBy rdf:resource="http://schema.org/"/>
        <rdfs:label xml:lang="es">región</rdfs:label>
    </owl:DatatypeProperty>
    


    <!-- http://schema.org/postalCode -->

    <owl:DatatypeProperty rdf:about="http://schema.org/postalCode">
        <rdfs:domain rdf:resource="http://schema.org/PostalAddress"/>
        <rdfs:range rdf:resource="http://www.w3.org/2001/XMLSchema#string"/>
        <rdfs:comment xml:lang="es">El código postal. Por ejemplo, 50071</rdfs:comment>
        <rdfs:isDefinedBy rdf:resource="http://schema.org/"/>
        <rdfs:label xml:lang="es">código postal</rdfs:label>
    </owl:DatatypeProperty>
    


    <!-- http://schema.org/streetAddress -->

    <owl:DatatypeProperty rdf:about="http://schema.org/streetAddress">
        <rdfs:domain rdf:resource="http://schema.org/PostalAddress"/>
        <rdfs:range rdf:resource="http://www.w3.org/2001/XMLSchema#string"/>
        <rdfs:comment xml:lang="es">La dirección de la calle. Por ejemplo, Vía Hispanidad, 20</rdfs:comment>
        <rdfs:isDefinedBy rdf:resource="http://schema.org/"/>
        <rdfs:label xml:lang="es">dirección</rdfs:label>
    </owl:DatatypeProperty>
    


    <!-- http://vocab.ciudadesabiertas.es/def/medio-ambiente/contaminacion-acustica#validada -->

    <owl:DatatypeProperty rdf:about="http://vocab.ciudadesabiertas.es/def/medio-ambiente/contaminacion-acustica#validada">
        <rdfs:domain rdf:resource="http://vocab.ciudadesabiertas.es/def/medio-ambiente/contaminacion-acustica#Observacion"/>
        <rdfs:range rdf:resource="http://www.w3.org/2001/XMLSchema#boolean"/>
    </owl:DatatypeProperty>
    


    <!-- http://vocab.linkeddata.es/datosabiertos/def/urbanismo-infraestructuras/equipamiento-municipal#fechaAlta -->

    <owl:DatatypeProperty rdf:about="http://vocab.linkeddata.es/datosabiertos/def/urbanismo-infraestructuras/equipamiento-municipal#fechaAlta">
        <rdfs:domain rdf:resource="http://vocab.linkeddata.es/datosabiertos/def/urbanismo-infraestructuras/equipamiento-municipal#Equipamiento"/>
        <rdfs:range rdf:resource="http://www.w3.org/2001/XMLSchema#date"/>
        <rdfs:isDefinedBy rdf:resource="http://vocab.linkeddata.es/datosabiertos/def/urbanismo-infraestructuras/equipamiento-municipal"/>
        <rdfs:label xml:lang="es">fecha de alta</rdfs:label>
        <rdfs:label xml:lang="en">start date</rdfs:label>
    </owl:DatatypeProperty>
    


    <!-- http://vocab.linkeddata.es/datosabiertos/def/urbanismo-infraestructuras/equipamiento-municipal#fechaBaja -->

    <owl:DatatypeProperty rdf:about="http://vocab.linkeddata.es/datosabiertos/def/urbanismo-infraestructuras/equipamiento-municipal#fechaBaja">
        <rdfs:domain rdf:resource="http://vocab.linkeddata.es/datosabiertos/def/urbanismo-infraestructuras/equipamiento-municipal#Equipamiento"/>
        <rdfs:range rdf:resource="http://www.w3.org/2001/XMLSchema#date"/>
        <rdfs:isDefinedBy rdf:resource="http://vocab.linkeddata.es/datosabiertos/def/urbanismo-infraestructuras/equipamiento-municipal"/>
        <rdfs:label xml:lang="en">end date</rdfs:label>
        <rdfs:label xml:lang="es">fecha de baja</rdfs:label>
    </owl:DatatypeProperty>
    


    <!-- http://www.w3.org/ns/sosa/hasSimpleResult -->

    <owl:DatatypeProperty rdf:about="http://www.w3.org/ns/sosa/hasSimpleResult"/>
    


    <!-- http://www.w3.org/ns/sosa/resultTime -->

    <owl:DatatypeProperty rdf:about="http://www.w3.org/ns/sosa/resultTime"/>
    


    <!-- https://schema.org/name -->

    <owl:DatatypeProperty rdf:about="https://schema.org/name">
        <rdfs:domain rdf:resource="http://vocab.linkeddata.es/datosabiertos/def/urbanismo-infraestructuras/equipamiento-municipal#Equipamiento"/>
        <rdfs:range rdf:resource="http://www.w3.org/2001/XMLSchema#string"/>
        <rdfs:comment xml:lang="es">Nombre del ítem</rdfs:comment>
        <rdfs:comment xml:lang="en">The name of the item</rdfs:comment>
        <rdfs:isDefinedBy rdf:resource="https://schema.org/"/>
        <rdfs:label xml:lang="en">name</rdfs:label>
        <rdfs:label xml:lang="es">nombre</rdfs:label>
    </owl:DatatypeProperty>
    


    <!-- 
    ///////////////////////////////////////////////////////////////////////////////////////
    //
    // Classes
    //
    ///////////////////////////////////////////////////////////////////////////////////////
     -->

    


    <!-- http://schema.org/PostalAddress -->

    <owl:Class rdf:about="http://schema.org/PostalAddress"/>
    


    <!-- http://vocab.ciudadesabiehttp://vocab.ciudadesabiertas.es/def/medio-ambiente/contaminacion-acustica#PropiedadContaminacion -->

    <owl:Class rdf:about="http://vocab.ciudadesabiehttp://vocab.ciudadesabiertas.es/def/medio-ambiente/contaminacion-acustica#PropiedadContaminacion">
        <rdfs:subClassOf rdf:resource="http://www.w3.org/ns/sosa/ObservableProperty"/>
        <rdfs:isDefinedBy rdf:resource="http://vocab.ciudadesabiertas.es/def/medio-ambiente/contaminacion-acustica"/>
    </owl:Class>
    


    <!-- http://vocab.ciudadesabiertas.es/def/medio-ambiente/contaminacion-acustica#EstacionMedida -->

    <owl:Class rdf:about="http://vocab.ciudadesabiertas.es/def/medio-ambiente/contaminacion-acustica#EstacionMedida">
        <rdfs:subClassOf rdf:resource="http://vocab.linkeddata.es/datosabiertos/def/urbanismo-infraestructuras/equipamiento-municipal#Equipamiento"/>
        <rdfs:subClassOf rdf:resource="http://www.w3.org/ns/sosa/Sensor"/>
        <rdfs:subClassOf>
            <owl:Restriction>
                <owl:onProperty rdf:resource="http://www.w3.org/ns/sosa/observes"/>
                <owl:allValuesFrom rdf:resource="http://vocab.ciudadesabiehttp://vocab.ciudadesabiertas.es/def/medio-ambiente/contaminacion-acustica#PropiedadContaminacion"/>
            </owl:Restriction>
        </rdfs:subClassOf>
        <rdfs:comment xml:lang="en">Device where the measurement of noise or vibration level is collected</rdfs:comment>
        <rdfs:comment xml:lang="es">Dispositivo donde se recoge la medida de nivel de ruido o vibración</rdfs:comment>
        <rdfs:isDefinedBy rdf:resource="http://vocab.ciudadesabiertas.es/def/medio-ambiente/contaminacion-acustica"/>
        <rdfs:label xml:lang="es">Estación de medida</rdfs:label>
        <rdfs:label xml:lang="en">Measuring station</rdfs:label>
    </owl:Class>
    


    <!-- http://vocab.ciudadesabiertas.es/def/medio-ambiente/contaminacion-acustica#Observacion -->

    <owl:Class rdf:about="http://vocab.ciudadesabiertas.es/def/medio-ambiente/contaminacion-acustica#Observacion">
        <rdfs:subClassOf rdf:resource="http://www.w3.org/ns/sosa/Observation"/>
        <rdfs:subClassOf>
            <owl:Restriction>
                <owl:onProperty rdf:resource="http://www.w3.org/ns/sosa/madeBySensor"/>
                <owl:allValuesFrom rdf:resource="http://vocab.ciudadesabiertas.es/def/medio-ambiente/contaminacion-acustica#EstacionMedida"/>
            </owl:Restriction>
        </rdfs:subClassOf>
        <rdfs:subClassOf>
            <owl:Restriction>
                <owl:onProperty rdf:resource="http://www.w3.org/ns/sosa/observedProperty"/>
                <owl:allValuesFrom rdf:resource="http://vocab.ciudadesabiehttp://vocab.ciudadesabiertas.es/def/medio-ambiente/contaminacion-acustica#PropiedadContaminacion"/>
            </owl:Restriction>
        </rdfs:subClassOf>
        <rdfs:isDefinedBy rdf:resource="http://vocab.ciudadesabiertas.es/def/medio-ambiente/contaminacion-acustica"/>
    </owl:Class>
    


    <!-- http://vocab.linkeddata.es/datosabiertos/def/urbanismo-infraestructuras/direccion-postal#DireccionPostal -->

    <owl:Class rdf:about="http://vocab.linkeddata.es/datosabiertos/def/urbanismo-infraestructuras/direccion-postal#DireccionPostal">
        <rdfs:subClassOf rdf:resource="http://schema.org/PostalAddress"/>
        <dct:issued rdf:datatype="http://www.w3.org/2001/XMLSchema#string">2014-03-28</dct:issued>
        <rdfs:comment xml:lang="es">Una dirección postal en España. Se define como una especialización de las clases vcard:Address, schema:PostalAddress y locn:Address
Además de las propiedades asociadas a estas clases, y definidas en su correspondiente vocabulario, también se pueden utilizar las definidas en los vocabularios de división administrativa española y en el callejero</rdfs:comment>
        <rdfs:isDefinedBy rdf:resource="http://vocab.linkeddata.es/datosabiertos/def/urbanismo-infraestructuras/direccion-postal"/>
        <rdfs:label xml:lang="es">Dirección postal</rdfs:label>
    </owl:Class>
    


    <!-- http://vocab.linkeddata.es/datosabiertos/def/urbanismo-infraestructuras/equipamiento-municipal#Equipamiento -->

    <owl:Class rdf:about="http://vocab.linkeddata.es/datosabiertos/def/urbanismo-infraestructuras/equipamiento-municipal#Equipamiento">
        <rdfs:subClassOf rdf:resource="http://www.opengis.net/spec/geosparql/1.0#Feature"/>
        <rdfs:subClassOf>
            <owl:Restriction>
                <owl:onProperty rdf:resource="http://vocab.linkeddata.es/datosabiertos/def/urbanismo-infraestructuras/equipamiento-municipal#fechaAlta"/>
                <owl:allValuesFrom rdf:resource="http://www.w3.org/2001/XMLSchema#date"/>
            </owl:Restriction>
        </rdfs:subClassOf>
        <rdfs:subClassOf>
            <owl:Restriction>
                <owl:onProperty rdf:resource="http://vocab.linkeddata.es/datosabiertos/def/urbanismo-infraestructuras/equipamiento-municipal#fechaBaja"/>
                <owl:allValuesFrom rdf:resource="http://www.w3.org/2001/XMLSchema#date"/>
            </owl:Restriction>
        </rdfs:subClassOf>
        <rdfs:subClassOf>
            <owl:Restriction>
                <owl:onProperty rdf:resource="https://schema.org/name"/>
                <owl:allValuesFrom rdf:resource="http://www.w3.org/2001/XMLSchema#string"/>
            </owl:Restriction>
        </rdfs:subClassOf>
        <rdfs:subClassOf>
            <owl:Restriction>
                <owl:onProperty rdf:resource="http://purl.org/dc/terms/identifier"/>
                <owl:qualifiedCardinality rdf:datatype="http://www.w3.org/2001/XMLSchema#nonNegativeInteger">1</owl:qualifiedCardinality>
                <owl:onDataRange rdf:resource="http://www.w3.org/2001/XMLSchema#string"/>
            </owl:Restriction>
        </rdfs:subClassOf>
        <rdfs:comment xml:lang="es">Equipamiento perteneciente a una administración, al que cualquier ciudadano puede acudir</rdfs:comment>
    </owl:Class>
    


    <!-- http://www.opengis.net/spec/geosparql/1.0#Feature -->

    <owl:Class rdf:about="http://www.opengis.net/spec/geosparql/1.0#Feature">
        <rdfs:comment xml:lang="en">This class represents the top-level feature type. This class is equivalent to GFI_Feature defined in ISO 19156, and it is superclass of all feature types.</rdfs:comment>
        <rdfs:isDefinedBy rdf:resource="http://www.opengis.net/spec/geosparql/1.0"/>
        <rdfs:label xml:lang="en">Feature</rdfs:label>
    </owl:Class>
    


    <!-- http://www.w3.org/2004/02/skos/core#Concept -->

    <owl:Class rdf:about="http://www.w3.org/2004/02/skos/core#Concept">
        <owl:disjointWith rdf:resource="http://www.w3.org/2004/02/skos/core#ConceptScheme"/>
        <dct:issued>2004-02-xx</dct:issued>
        <rdfs:isDefinedBy rdf:resource="http://www.w3.org/2004/02/skos/core#"/>
        <rdfs:label xml:lang="en">Concept</rdfs:label>
        <skos:definition>An abstract idea or notion; a unit of thought.</skos:definition>
    </owl:Class>
    


    <!-- http://www.w3.org/2004/02/skos/core#ConceptScheme -->

    <owl:Class rdf:about="http://www.w3.org/2004/02/skos/core#ConceptScheme">
        <dct:issued>2004-02-xx</dct:issued>
        <rdfs:comment xml:lang="en">A concept scheme may be defined to include concepts from different sources.</rdfs:comment>
        <rdfs:comment xml:lang="en">Thesauri, classification schemes, subject heading lists, taxonomies, &apos;folksonomies&apos;, and other types of controlled vocabulary are all examples of concept schemes.  Concept schemes are also embedded in glossaries and terminologies.</rdfs:comment>
        <rdfs:isDefinedBy rdf:resource="http://www.w3.org/2004/02/skos/core#"/>
        <rdfs:label xml:lang="en">Concept Scheme</rdfs:label>
        <skos:definition xml:lang="en">A set of concepts, optionally including statements about semantic relationships between those concepts.</skos:definition>
    </owl:Class>
    


    <!-- http://www.w3.org/ns/sosa/ObservableProperty -->

    <owl:Class rdf:about="http://www.w3.org/ns/sosa/ObservableProperty"/>
    


    <!-- http://www.w3.org/ns/sosa/Observation -->

    <owl:Class rdf:about="http://www.w3.org/ns/sosa/Observation">
        <rdfs:subClassOf>
            <owl:Restriction>
                <owl:onProperty rdf:resource="http://www.w3.org/ns/sosa/hasSimpleResult"/>
                <owl:cardinality rdf:datatype="http://www.w3.org/2001/XMLSchema#nonNegativeInteger">1</owl:cardinality>
            </owl:Restriction>
        </rdfs:subClassOf>
        <rdfs:subClassOf>
            <owl:Restriction>
                <owl:onProperty rdf:resource="http://www.w3.org/ns/sosa/resultTime"/>
                <owl:qualifiedCardinality rdf:datatype="http://www.w3.org/2001/XMLSchema#nonNegativeInteger">1</owl:qualifiedCardinality>
                <owl:onDataRange rdf:resource="http://www.w3.org/2001/XMLSchema#dateTime"/>
            </owl:Restriction>
        </rdfs:subClassOf>
    </owl:Class>
    


    <!-- http://www.w3.org/ns/sosa/Sensor -->

    <owl:Class rdf:about="http://www.w3.org/ns/sosa/Sensor"/>
    


    <!-- 
    ///////////////////////////////////////////////////////////////////////////////////////
    //
    // Individuals
    //
    ///////////////////////////////////////////////////////////////////////////////////////
     -->

    


    <!-- http://vocab.ciudadesabiertas.es/def/medio-ambiente/contaminacion-acustica#nivelRuido -->

    <owl:NamedIndividual rdf:about="http://vocab.ciudadesabiertas.es/def/medio-ambiente/contaminacion-acustica#nivelRuido">
        <rdf:type rdf:resource="http://vocab.ciudadesabiehttp://vocab.ciudadesabiertas.es/def/medio-ambiente/contaminacion-acustica#PropiedadContaminacion"/>
        <rdfs:label xml:lang="es">nivel de ruido</rdfs:label>
        <rdfs:label xml:lang="en">noise level</rdfs:label>
    </owl:NamedIndividual>
    


    <!-- http://vocab.ciudadesabiertas.es/def/medio-ambiente/contaminacion-acustica#nivelVibracion -->

    <owl:NamedIndividual rdf:about="http://vocab.ciudadesabiertas.es/def/medio-ambiente/contaminacion-acustica#nivelVibracion">
        <rdf:type rdf:resource="http://vocab.ciudadesabiehttp://vocab.ciudadesabiertas.es/def/medio-ambiente/contaminacion-acustica#PropiedadContaminacion"/>
        <rdfs:label xml:lang="es">nivel de vibración</rdfs:label>
        <rdfs:label xml:lang="en">vibration level</rdfs:label>
    </owl:NamedIndividual>
    


    <!-- http://vocab.linkeddata.es/datosabiertos/kos/medio-ambiente/contaminacion-acustica/tipo-emisor-predominante -->

    <owl:NamedIndividual rdf:about="http://vocab.linkeddata.es/datosabiertos/kos/medio-ambiente/contaminacion-acustica/tipo-emisor-predominante">
        <rdf:type rdf:resource="http://www.w3.org/2004/02/skos/core#ConceptScheme"/>
    </owl:NamedIndividual>
    


    <!-- http://vocab.linkeddata.es/datosabiertos/kos/medio-ambiente/contaminacion-acustica/tipo-intervalo-referencia -->

    <owl:NamedIndividual rdf:about="http://vocab.linkeddata.es/datosabiertos/kos/medio-ambiente/contaminacion-acustica/tipo-intervalo-referencia">
        <rdf:type rdf:resource="http://www.w3.org/2004/02/skos/core#ConceptScheme"/>
    </owl:NamedIndividual>
    


    <!-- http://vocab.linkeddata.es/datosabiertos/kos/medio-ambiente/contaminacion-acustica/tipo-medicion -->

    <owl:NamedIndividual rdf:about="http://vocab.linkeddata.es/datosabiertos/kos/medio-ambiente/contaminacion-acustica/tipo-medicion">
        <rdf:type rdf:resource="http://www.w3.org/2004/02/skos/core#ConceptScheme"/>
    </owl:NamedIndividual>
    


    <!-- http://vocab.linkeddata.es/datosabiertos/kos/urbanismo-infraestructuras/equipamiento/tipo-equipamiento -->

    <owl:NamedIndividual rdf:about="http://vocab.linkeddata.es/datosabiertos/kos/urbanismo-infraestructuras/equipamiento/tipo-equipamiento">
        <rdf:type rdf:resource="http://www.w3.org/2004/02/skos/core#ConceptScheme"/>
    </owl:NamedIndividual>
    


    <!-- 
    ///////////////////////////////////////////////////////////////////////////////////////
    //
    // Annotations
    //
    ///////////////////////////////////////////////////////////////////////////////////////
     -->

    <rdf:Description rdf:about="http://www.w3.org/ns/sosa/hasSimpleResult">
        <skos:example xml:lang="en">For instance, the values 23 or true.</skos:example>
        <rdfs:comment xml:lang="en">The simple value of an Observation or Actuation or act of Sampling.</rdfs:comment>
        <rdfs:isDefinedBy rdf:resource="http://www.w3.org/ns/sosa/"/>
        <schema:domainIncludes rdf:resource="http://www.w3.org/ns/sosa/Actuation"/>
        <schema:domainIncludes rdf:resource="http://www.w3.org/ns/sosa/Observation"/>
        <rdfs:label xml:lang="en">has simple result</rdfs:label>
        <skos:definition xml:lang="en">The simple value of an Observation or Actuation or act of Sampling.</skos:definition>
        <schema:domainIncludes rdf:resource="http://www.w3.org/ns/sosa/Sampling"/>
    </rdf:Description>
    <rdf:Description rdf:about="http://www.w3.org/ns/sosa/resultTime">
        <rdfs:isDefinedBy rdf:resource="http://www.w3.org/ns/sosa/"/>
        <schema:domainIncludes rdf:resource="http://www.w3.org/ns/sosa/Actuation"/>
        <rdfs:label xml:lang="en">result time</rdfs:label>
        <schema:domainIncludes rdf:resource="http://www.w3.org/ns/sosa/Observation"/>
        <schema:domainIncludes rdf:resource="http://www.w3.org/ns/sosa/Sampling"/>
        <rdfs:comment xml:lang="en">The result time is the instant of time when the Observation, Actuation or Sampling activity was completed.</rdfs:comment>
        <skos:definition xml:lang="en">The result time is the instant of time when the Observation, Actuation or Sampling activity was completed.</skos:definition>
    </rdf:Description>
</rdf:RDF>



<!-- Generated by the OWL API (version 4.2.6.20160910-2108) https://github.com/owlcs/owlapi -->

